Metatheory.lean
@@ -76,6 +76,7 @@ import Metatheory.ResourceLogic
 import Metatheory.Rewriting.Basic
 import Metatheory.Rewriting.Compat
 import Metatheory.Rewriting.DecreasingDiagrams
+import Metatheory.Rewriting.DecreasingDiagramsCertificate
 import Metatheory.Rewriting.DecreasingDiagramsExample
 import Metatheory.Rewriting.DecreasingDiagramsFamily
 import Metatheory.Rewriting.Diamond
